## Exercise 4.1.4

Suppose $G$ is an arbitrary operator, so
$$
(G^{\dagger}G)^{\dagger} = G^{\dagger}G, (GG^{\dagger})^{\dagger} = GG^{\dagger}\tag{1}
$$
Then $G^{\dagger}G$ and $GG^{\dagger}$ are a Hermitian operator. The function $f: V\rightarrow V$ for a Hermitian operator $A$ is defined by
$$
f(A) = \sum_{i}f(\lambda_{i})|i\rangle\langle i|\tag{2}
$$
 where $\{|i\rangle \}$â€‹ is a set of orthonormal basis. 
$$
f(G^{\dagger}G) = \sum_{i}f(v_{i})|i\rangle\langle i|\\
f(GG^{\dagger}) = \sum_{j}f(w_{j})|j\rangle\langle j|
$$
...
