## Exercise 3.3.2

The matrix representation of $X$ and $Z$ in the basis $\{|0\rangle, |1\rangle\}$ are given by
$$
X = \begin{pmatrix}
0 & 1\\ 1 &0
\end{pmatrix},Z = \begin{pmatrix}
1 & 0\\ 0 &-1
\end{pmatrix}\tag{1}
$$
Thus, the matrix representation for $[X, Z]$ are given by
$$
\begin{align}
[X, Z] = XZ-ZX &=\begin{pmatrix}
0 & 1\\ 1 &0
\end{pmatrix}\begin{pmatrix}
1 & 0\\ 0 &-1
\end{pmatrix} - \begin{pmatrix}
1 & 0\\ 0 &-1
\end{pmatrix}\begin{pmatrix}
0 & 1\\ 1 &0
\end{pmatrix} \\
&= \begin{pmatrix}
0 & -1\\ 1 &0
\end{pmatrix} -\begin{pmatrix}
0 & 1\\ -1 & 0
\end{pmatrix} = \begin{pmatrix}
0 & -2\\ 2 & 0
\end{pmatrix}
\end{align}\tag{2}
$$
