## Exercise 3.3.11

Suppose that $A$ is Hermitian and it can be decomposed into the form 
$$
A = \sum_{i} a_{1}|i\rangle\langle i| \tag{1}\label{1}
$$
where $|i\rangle$ is a set of orthonormal basis, the function of an operator $A$​​ is defined by
$$
f(A) = \sum_{i}f(a_i)|i\rangle\langle i|\tag{2}\label{2}
$$
Also, for sine and cosine function, we have
$$
\cos\frac{\phi}{2} = \frac{e^{i\phi/2}+ e^{-i\phi/2}}{2}, \sin\frac{\phi}{2} = \frac{e^{i\phi/2}- e^{-i\phi/2}}{2i}\tag{3}\label{3}
$$
Here I will use eq. $\eqref{1}-\eqref{3}$ to prove the rotation operator expression. 

* For $R_{X}(\phi) = \exp \{iX\phi/2\}$, since $|+\rangle$ and $|-\rangle$ are eigenvector of $X$ With eigenvalue $+1$ and $-1$, respectively, we can write $X$ into the form as eq. $\eqref{1}$,
  $$
  \begin{align}
  X &= |+\rangle\langle +| - |-\rangle\langle -|  \\
  &= \frac{1}{2}\begin{pmatrix}
  1 \\ 1 
  \end{pmatrix}\begin{pmatrix}
  1 & 1 
  \end{pmatrix} - \frac{1}{2}\begin{pmatrix}
  1 \\ -1 
  \end{pmatrix}\begin{pmatrix}
  1 & -1 
  \end{pmatrix}\\
  &= \frac{1}{2}\begin{pmatrix}
  1 & 1 \\ 1 & 1
  \end{pmatrix} - \frac{1}{2}\begin{pmatrix}
  1 & -1 \\ -1 & 1
  \end{pmatrix}\\
  &= \begin{pmatrix}
  0 & 1 \\ 1 & 0
  \end{pmatrix}
  \end{align}\tag{4}
  $$
  According to eq. $\eqref{2}$, the rotation operator is then given by
  $$
  \exp \{iX\phi/2\} = e^{i\phi/2}|+\rangle\langle +| + e^{-i\phi/2}|-\rangle\langle -|\tag{5}\label{5}
  $$
  Note that 
  $$
  \begin{align}
  |+\rangle\langle +| &= \frac{1}{2}\begin{pmatrix}
  1 & 1 \\ 1 & 1
  \end{pmatrix} = \frac{1}{2}(I+X)\tag{6a}\label{6a}\\
  |-\rangle\langle -| &= \frac{1}{2}\begin{pmatrix}
  1 & -1 \\ -1 & 1
  \end{pmatrix} = \frac{1}{2}(I-X)\tag{6b}\label{6b}
  \end{align}
  $$
  Use eq. $\eqref{6a}-\eqref{6b}$, we can re-write eq. $\eqref{5}$​ as
  $$
  \begin{align}
  \exp \{iX\phi/2\} &= e^{i\phi/2}|+\rangle\langle +| + e^{-i\phi/2}|-\rangle\langle -| \\
  &= \frac{1}{2}e^{i\phi/2}(I+X) + \frac{1}{2}e^{-i\phi/2}(I-X) 
  \end{align}\tag{7}\label{7}
  $$
  Use eq. $\eqref{3}$​, we can re-write eq. $\eqref{7}$​ as
  $$
  \begin{align}
  \exp \{iX\phi/2\} &= \frac{1}{2}e^{i\phi/2}(I+X) + \frac{1}{2}e^{-i\phi/2}(I-X) \\
  &= \frac{1}{2}(e^{i\phi/2}+e^{-i\phi/2})I + \frac{1}{2i}(e^{i\phi/2}-e^{-i\phi/2})iX \\
  &= \cos\frac{\phi}{2} I + i\sin\frac{\phi}{2} X
  \end{align}\tag{8}\label{8}
  $$

* For $R_{Y}(\phi) = \exp \{iY\phi/2\}$​​, since
  $$
  |\psi\rangle = \frac{1}{\sqrt{2}}\begin{pmatrix}
  1 \\ i
  \end{pmatrix}, |\phi\rangle = \frac{1}{\sqrt{2}}\begin{pmatrix}
  1\\ -i
  \end{pmatrix}\tag{9}
  $$
  are eigenvector of $Y$ with eigenvalue $+1$ and $-1$, respectively, we can write $Y$ into the form as eq. $\eqref{1}$​​,
  $$
  \begin{align}
  Y &= |\psi\rangle\langle \psi| - |\phi\rangle\langle \phi|  \\
  &= \frac{1}{2}\begin{pmatrix}
  1 \\ i
  \end{pmatrix}\begin{pmatrix}
  1 & -i 
  \end{pmatrix} - \frac{1}{2}\begin{pmatrix}
  1 \\ -i 
  \end{pmatrix}\begin{pmatrix}
  1 & i 
  \end{pmatrix}\\
  &= \frac{1}{2}\begin{pmatrix}
  1 & -i \\ i & 1
  \end{pmatrix} - \frac{1}{2}\begin{pmatrix}
  1 & i \\ -i & 1
  \end{pmatrix}\\
  &= \begin{pmatrix}
  0 & -i \\ i & 0
  \end{pmatrix}
  \end{align}\tag{10}
  $$
  According to eq. $\eqref{2}$, the rotation operator is then given by
  $$
  \exp \{iY\phi/2\} = e^{i\phi/2}|\psi\rangle\langle \psi| + e^{-i\phi/2}|\phi\rangle\langle \phi|\tag{11}\label{11}
  $$
  Note that 
  $$
  \begin{align}
  |\psi\rangle\langle \psi| &= \frac{1}{2}\begin{pmatrix}
  1 & -i \\ i & 1
  \end{pmatrix} = \frac{1}{2}(I+Y)\tag{12a}\label{12a}\\
  |\phi\rangle\langle \phi| &= \frac{1}{2}\begin{pmatrix}
  1 & i \\ -i & 1
  \end{pmatrix} = \frac{1}{2}(I-Y)\tag{12b}\label{12b}
  \end{align}
  $$
  Use eq. $\eqref{12a}-\eqref{12b}$, we can re-write eq. $\eqref{11}$​ as
  $$
  \begin{align}
  \exp \{iY\phi/2\} &= e^{i\phi/2}|\psi\rangle\langle \psi| + e^{-i\phi/2}|\phi\rangle\langle \phi| \\
  &= \frac{1}{2}e^{i\phi/2}(I+Y) + \frac{1}{2}e^{-i\phi/2}(I-Y) 
  \end{align}\tag{13}\label{13}
  $$
  Use eq. $\eqref{3}$​​, we can re-write eq. $\eqref{13}$​​ as
  $$
  \begin{align}\exp \{iY\phi/2\} &= \frac{1}{2}e^{i\phi/2}(I+Y) + \frac{1}{2}e^{-i\phi/2}(I-Y) \\&= \frac{1}{2}(e^{i\phi/2}+e^{-i\phi/2})I + \frac{1}{2i}(e^{i\phi/2}-e^{-i\phi/2})iY \\&= \cos\frac{\phi}{2} I + i\sin\frac{\phi}{2} Y\end{align}\tag{14}\label{14}
  $$

* For $R_{Z}(\phi) = \exp \{iZ\phi/2\}$, since $|0\rangle$ and $|1\rangle$ are eigenvector of $Z$ With eigenvalue $+1$ and $-1$, respectively, we can write $Z$ into the form as eq. $\eqref{1}$,
  $$
  \begin{align}
  Z &= |0\rangle\langle 0| - |1\rangle\langle 1|  \\
  &= \begin{pmatrix}
  1 \\ 0
  \end{pmatrix}\begin{pmatrix}
  1 & 0
  \end{pmatrix} - \begin{pmatrix}
  0 \\ 1 
  \end{pmatrix}\begin{pmatrix}
  0 & 1
  \end{pmatrix}\\
  &= \begin{pmatrix}
  1 & 0 \\ 0 & 0
  \end{pmatrix} - \begin{pmatrix}
  0 & 0 \\ 0 & 1
  \end{pmatrix}\\
  &= \begin{pmatrix}
  1 & 0 \\ 0 & -1
  \end{pmatrix}
  \end{align}\tag{15}
  $$
  According to eq. $\eqref{2}$, the rotation operator is then given by
  $$
  \exp \{iZ\phi/2\} = e^{i\phi/2}|0\rangle\langle 0| + e^{-i\phi/2}|1\rangle\langle 1|\tag{16}\label{16}
  $$
  Note that 
  $$
  \begin{align}
  |0\rangle\langle 0| &= \begin{pmatrix}
  1 & 0 \\ 0 & 0
  \end{pmatrix} = \frac{1}{2}(I+Z)\tag{17a}\label{17a}\\
  |1\rangle\langle 1| &= \begin{pmatrix}
  0 & 0 \\ 0 & 1
  \end{pmatrix} = \frac{1}{2}(I-X)\tag{17b}\label{17b}
  \end{align}
  $$
  Use eq. $\eqref{17a}-\eqref{17b}$, we can re-write eq. $\eqref{16}$​ as
  $$
  \begin{align}
  \exp \{iZ\phi/2\} &= e^{i\phi/2}|+\rangle\langle +| + e^{-i\phi/2}|-\rangle\langle -| \\
  &= \frac{1}{2}e^{i\phi/2}(I+Z) + \frac{1}{2}e^{-i\phi/2}(I-Z) 
  \end{align}\tag{18}\label{18}
  $$
  Use eq. $\eqref{3}$​​, we can re-write eq. $\eqref{18}$​​ as
  $$
  \begin{align}
  \exp \{iZ\phi/2\} &= \frac{1}{2}e^{i\phi/2}(I+Z) + \frac{1}{2}e^{-i\phi/2}(I-Z) \\&= \frac{1}{2}(e^{i\phi/2}+e^{-i\phi/2})I + \frac{1}{2i}(e^{i\phi/2}-e^{-i\phi/2})iZ \\&= \cos\frac{\phi}{2} I + i\sin\frac{\phi}{2} Z
  \end{align}\tag{19}\label{19}
  $$

From eq. $\eqref{8}$, eq. $\eqref{14}$ and eq. $\eqref{19}$, we can conclude that
$$
\begin{align}
\exp \{iX\phi/2\} &= \cos\frac{\phi}{2} I + i\sin\frac{\phi}{2} X \tag{20a}\\
\exp \{iY\phi/2\} &= \cos\frac{\phi}{2} I + i\sin\frac{\phi}{2} Y \tag{20b}\\
\exp \{iZ\phi/2\} &= \cos\frac{\phi}{2} I + i\sin\frac{\phi}{2} Z \tag{20c}\\
\end{align}
$$
